wip ***NO_CI***

examples/crypto/EtM.AE.fst
@@ -19,7 +19,8 @@ abstract type cipher = (CPA.cipher * MAC.tag)
 
 type rid = FStar.Monotonic.Seq.rid
 
-type log_t (r:rid) = m_rref r (seq (CPA.msg * cipher)) grows
+let log_entry = CPA.msg * cipher
+type log_t (r:rid) = m_rref r (seq log_entry) grows
 
 noeq type key =
   | Key:  #region:rid ->
@@ -37,6 +38,23 @@ let get_mac_log (h:mem) (k:key) =
 let get_cpa_log (h:mem) (k:key) =
   m_sel h (CPA.Key?.log k.ke)
 
+//Only valid ciphers are mac'd
+let mac_only_cpa_ciphers (mac:Seq.seq EtM.MAC.log_entry) (cpa:Seq.seq EtM.CPA.log_entry) =
+  forall (c:cipher). {:pattern (Seq.mem c mac)}
+     Seq.mem c mac
+      <==>
+     (exists (p:Plain.plain). Seq.mem (CPA.Entry p (fst c)) cpa)
+
+//AE log abstracts the mac and cpa logs
+let mac_and_cpa_refine_ae (ae:Seq.seq log_entry) 
+                          (mac:Seq.seq EtM.MAC.log_entry)
+                          (cpa:Seq.seq EtM.CPA.log_entry) =
+  forall (p:Plain.plain) (c:cipher).{:pattern (Seq.mem (p, c) ae)}
+     Seq.mem (p,c) ae
+     <==>
+     (Seq.mem c mac /\
+      Seq.mem (CPA.Entry p (fst c)) cpa)
+
 let invariant (h:mem) (k:key) =
   let log = get_log h k in
   let mac_log = get_mac_log h k in
@@ -46,41 +64,9 @@ let invariant (h:mem) (k:key) =
   Map.contains h.h (CPA.Key?.region k.ke) /\
   Seq.length log = Seq.length mac_log /\
   Seq.length mac_log = Seq.length cpa_log /\
-  //Only valid ciphers are mac'd
-  (forall (c:cipher). {:pattern (Seq.mem c (get_mac_log h k))}
-     Seq.mem c (get_mac_log h k)
-      <==>
-     (exists (p:Plain.plain). Seq.mem (p, fst c) (get_cpa_log h k))) /\
-  //The AE log abstracts the mac and cpa logs     
-  (forall (p:Plain.plain) (c:cipher).{:pattern (Seq.mem (p, c) (get_log h k))}
-     Seq.mem (p,c) (get_log h k)
-     <==>
-     (Seq.mem c (get_mac_log h k) /\
-      Seq.mem (p, fst c) (get_cpa_log h k)))
-
-let test (k:key) (c:cipher) (h:mem) : 
-  Lemma (requires (invariant h k /\
-                   Seq.mem c (get_mac_log h k)))
-        (ensures  (Some? (seq_find (fun mc -> snd mc = c) (get_cpa_log h k))))
-  = ()        
-        
-  //   (
-  // (forall (i:int).{:pattern (Seq.index log i)}
-  //   indexable log i ==>
-  //   (let cipher,tag = Seq.index mac_log i in
-  //    let plain,cipher' = Seq.index cpa_log i in
-  //    cipher = cipher' /\
-  //    Seq.index log i == (plain,(cipher,tag))
-  //   )
-  // )
-
-let invariant_mem (k:key) (c:cipher) (p:Plain.plain) (h:mem)
-    : Lemma 
-    (requires (invariant h k /\
-               Seq.mem c (get_mac_log h k) /\
-               Seq.mem (p, fst c) (get_cpa_log h k)))
-    (ensures (Seq.mem (p, c) (get_log h k)))
-    = ()
+  EtM.CPA.invariant (Key?.ke k) h /\
+  mac_only_cpa_ciphers (get_mac_log h k) (get_cpa_log h k) /\
+  mac_and_cpa_refine_ae (get_log h k) (get_mac_log h k) (get_cpa_log h k)
 
 let genPost parent h0 (k:key) h1 =
     modifies Set.empty h0 h1
@@ -108,15 +94,19 @@ val encrypt: k:key -> m:Plain.plain -> ST cipher
     (let log0 = get_log h0 k in
      let log1 = get_log h1 k in
      HyperHeap.modifies (Set.singleton k.region)  h0.h h1.h
-     /\ log1 == snoc log0 (m, c)
-     /\ witnessed (at_least (Seq.length log0) (m, c) k.log)
-     /\ invariant h1 k)))
+     /\ invariant h1 k
+     /\ log1 == snoc log0 (m, c))))
+     
+     // /\ witnessed (at_least (Seq.length log0) (m, c) k.log)
+     // /\ invariant h1 k)))
 
 // #set-options "--initial_fuel 0 --max_fuel 0 --initial_ifuel 1 --max_ifuel 1 --z3rlimit 100"
 let encrypt k plain =
   let c = CPA.encrypt k.ke plain in
   let t = MAC.mac k.km c in
   write_at_end k.log (plain, (c, t));
+  let h = FStar.HyperStack.ST.get () in
+  assert (EtM.CPA.invariant (Key?.ke k) h);
   admit();
   (c, t)
 
@@ -125,24 +115,10 @@ val decrypt: k:key -> c:cipher -> ST (option Plain.plain)
   (ensures (fun h0 res h1 ->
     modifies_none h0 h1 /\
     invariant h1 k /\
-    (Ideal.uf_cma /\ Some? res ==>
+    (b2t Ideal.uf_cma /\ Some? res ==>
      Seq.mem (Some?.v res, c) (get_log h0 k))))
-         
-//         (Some? (seq_find (fun (m,c') -> m = Some?.v res && c = c') (get_log h0 k)))
-// (* CH*MK: If we wanted to also prove correctness of the EtM.AE
-//           we would use this stronger post-condition:
-//         Seq.mem (Some.v res, c) (m_sel h0 k.log) *)
-//       )
-//   ))
-
 let decrypt k (c,tag) =
-  // assume (b2t (Ideal.uf_cma));
-  let h = FStar.HyperStack.ST.get () in
   if MAC.verify k.km c tag
   then let msg = CPA.decrypt k.ke c in
-       let _ = admit() in
        Some msg
-        // assert (Seq.mem (msg, c) (get_cpa_log h k));
-        // invariant_mem k (c, tag) msg h;
-        // Some msg)
   else None
